Filesys/PathBasedFSInv.i.dfy
@@ -1,0 +1,190 @@
+// Copyright 2018-2021 VMware, Inc., Microsoft Inc., Carnegie Mellon University, ETH Zurich, and University of Washington
+// SPDX-License-Identifier: BSD-2-Clause
+include "PathBasedFS.i.dfy"
+
+module PathBasedFSInv {
+  import opened Options
+  import opened PathBasedFS
+  import opened FSTypes
+  import opened PathSpec
+
+  predicate Inv(fs: FileSys)
+  {
+    && WF(fs)
+    // path is connected
+    && (forall path | PathExists(fs, path) && path != RootDir :: ParentDirIsDir(fs, path))
+    // redirect meta points to a valid and hidden path meta
+    && (forall path | fs.meta_map[path].RedirectMeta? :: 
+        && fs.meta_map[fs.meta_map[path].source].PathMeta?
+        && fs.meta_map[fs.meta_map[path].source].hidden
+        && !fs.meta_map[fs.meta_map[path].source].m.ftype.Directory?)
+  }
+
+  lemma InitImpliesInv(fs: FileSys)
+  requires Init(fs)
+  ensures Inv(fs)
+  {
+  }
+
+  lemma NextPreservesInv(fs: FileSys, fs': FileSys)
+  requires Inv(fs)
+  requires Next(fs, fs')
+  ensures Inv(fs')
+  {
+    var step :| NextStep(fs, fs', step);
+    NextStepPreservesInv(fs, fs', step);
+  }
+
+  lemma NextStepPreservesInv(fs: FileSys, fs': FileSys, step: Step)
+  requires Inv(fs)
+  requires NextStep(fs, fs', step)
+  ensures Inv(fs')
+  {
+    match step {
+      case DeleteStep(path, ctime) => DeletePreservesInv(fs, fs', path, ctime);
+      case RenameStep(source, dest, ctime) => RenamePreservesInv(fs, fs', source, dest, ctime);
+      case LinkStep(source, dest, ctime, hiddenName) => LinkPreservesInv(fs, fs', source, dest, ctime, hiddenName);
+      case _ => {
+        if step.CreateStep? || step.ChangeAttrStep? || step.TruncateStep? || step.WriteStep? || step.UpdateTimeStep? {
+          SimpleStepPreservesInv(fs, fs', step);
+        }
+      }
+    }
+  }
+
+  lemma DeletePreservesInv(fs: FileSys, fs': FileSys, path: Path, ctime: Time)
+  requires Inv(fs)
+  requires Delete(fs, fs', path, ctime)
+  ensures Inv(fs')
+  {
+    forall p | PathExists(fs', p) && p != RootDir
+    ensures ParentDirIsDir(fs', p)
+    {
+      assert PathExists(fs, p); // observe
+    }
+
+    // forall p | fs'.meta_map[p].RedirectMeta? 
+    // ensures fs'.meta_map[fs'.meta_map[p].source].PathMeta?
+    // ensures fs'.meta_map[fs'.meta_map[p].source].hidden
+    // ensures !fs'.meta_map[fs'.meta_map[p].source].m.ftype.Directory?
+    // {
+    //   var m := fs.meta_map[path];
+
+    //   if m.RedirectMeta? && fs'.meta_map[p].source == m.source {
+    //     assert fs.meta_map[p] == fs'.meta_map[p];
+    //     assert fs'.meta_map[m.source] == MetaDataDelete(fs, path, ctime);
+
+    //     if NoAlias(fs, path) {
+    //       assert p != path;
+    //       assert false;
+    //     }
+    //   }
+    // }
+    assert Inv(fs');
+  }
+
+  // lemma RenamedPathsRemainDifferent(src: Path, dst: Path, p1: Path, p2: Path)
+  // requires p1 != p2
+  // requires p1 == dst || BeneathDir(dst, p1)
+  // requires p2 == dst || BeneathDir(dst, p2)
+  // ensures src + p1[|dst|..] != src + p2[|dst|..]
+  // {
+  //   if BeneathDir(dst, p1) && BeneathDir(dst, p2) {
+  //     assert p1[|dst|..] != p2[|dst|..];
+
+  //     var p1' := src + p1[|dst|..];
+  //     var p2' := src + p2[|dst|..];
+
+  //     assert p1'[..|src|] == p2'[..|src|];
+  //   }
+  // }
+
+  lemma {:timeLimitMultiplier 2} RenamePreservesInv(fs: FileSys, fs': FileSys, src: Path, dst: Path, ctime: Time)
+  requires Inv(fs)
+  requires Rename(fs, fs', src, dst, ctime)
+  ensures Inv(fs')
+  {
+    forall p | PathExists(fs', p) && p != RootDir
+    ensures ParentDirIsDir(fs', p)
+    {
+      if p == dst {
+        assert ParentDirIsDir(fs', p);
+      } else if BeneathDir(dst, p) {
+        var parent_dir := GetParentDir(p);
+        var srcpath := src + p[|dst|..];
+        var srcparent_dir := GetParentDir(srcpath);
+        assert ParentDirIsDir(fs, srcpath); // observe
+        assert parent_dir == dst || BeneathDir(dst, parent_dir); // observe
+
+        if parent_dir == dst {
+          assert fs'.meta_map[parent_dir] == UpdatePathCtime(fs, src, ctime);
+        } else {
+          assert src + parent_dir[|dst|..] == srcparent_dir; // observe
+          assert fs'.meta_map[parent_dir] == fs.meta_map[srcparent_dir];
+        }
+      } else if fs.meta_map[dst].RedirectMeta? && fs.meta_map[dst].source == p {
+        assert ParentDirIsDir(fs', p);
+      } else if  p == GetParentDir(src) || p == GetParentDir(dst) {
+        assert ParentDirIsDir(fs', p);
+      } else {
+        assert ParentDirIsDir(fs, p);
+        assert ParentDirIsDir(fs', p);
+      }
+    }
+
+    forall p | fs'.meta_map[p].RedirectMeta? 
+    ensures fs'.meta_map[fs'.meta_map[p].source].PathMeta?
+    ensures fs'.meta_map[fs'.meta_map[p].source].hidden
+    ensures !fs'.meta_map[fs'.meta_map[p].source].m.ftype.Directory?
+    {
+      assume false;
+      // if (p == dest || p == source) && fs.meta_map[source].PathMeta? {
+      //   assert fs'.meta_map[hiddenName.value] == LinkMeta(fs, source, ctime);
+      // }
+    }
+    assert Inv(fs');
+  }
+
+  lemma LinkPreservesInv(fs: FileSys, fs': FileSys, source: Path, dest: Path, ctime: Time, hiddenName: Option<Path>)
+  requires Inv(fs)
+  requires Link(fs, fs', source, dest, ctime, hiddenName)
+  ensures Inv(fs')
+  {
+    forall p | PathExists(fs', p) && p != RootDir
+    ensures ParentDirIsDir(fs', p)
+    {
+      if p == dest {
+        assert ParentDirIsDir(fs', p);
+      } else {
+        assert PathExists(fs, p); // observe
+      }
+    }
+
+    forall p | fs'.meta_map[p].RedirectMeta? 
+    ensures fs'.meta_map[fs'.meta_map[p].source].PathMeta?
+    ensures fs'.meta_map[fs'.meta_map[p].source].hidden
+    ensures !fs'.meta_map[fs'.meta_map[p].source].m.ftype.Directory?
+    {
+      if (p == dest || p == source) && fs.meta_map[source].PathMeta? {
+        assert fs'.meta_map[hiddenName.value] == LinkMeta(fs, source, ctime);
+      }
+    }
+    assert Inv(fs');
+  }
+
+  lemma SimpleStepPreservesInv(fs: FileSys, fs': FileSys, step: Step)
+  requires Inv(fs)
+  requires NextStep(fs, fs', step)
+  requires step.CreateStep? || step.ChangeAttrStep? || step.TruncateStep? || step.WriteStep? || step.UpdateTimeStep?
+  ensures Inv(fs')
+  {
+    forall p | PathExists(fs', p) && p != RootDir 
+    ensures ParentDirIsDir(fs', p)
+    {
+      if p != step.path {
+        assert PathExists(fs, p); // observe
+      }
+    }
+    assert Inv(fs');
+  }
+}
